one admit left

theories/FOL/Reductions/PCPb_to_ZFeq.v
@@ -98,14 +98,48 @@ Section ZF.
     apply (@M_ZF (fun _ => ∅) ax_pair). cbn; tauto.
   Qed.
 
+  Definition pair x y :=
+    {x; y}.
+
+  Instance set_equiv_pair :
+    Proper (set_equiv ==> set_equiv ==> set_equiv) pair.
+  Proof.
+    intros x x' Hx y y' Hy. unfold pair.
+    apply M_ext; unfold set_sub.
+    all: setoid_rewrite M_pair.
+    all: setoid_rewrite Hx; setoid_rewrite Hy; tauto.
+  Qed.
+
+  Instance set_equiv_opair :
+    Proper (set_equiv ==> set_equiv ==> set_equiv) M_opair.
+  Proof.
+    intros x x' Hx y y' Hy. unfold M_opair.
+    change ({pair x x; pair x y} ≡' {pair x' x'; pair x' y'}).
+    apply M_ext; unfold set_sub.
+    all: setoid_rewrite M_pair.
+    all: setoid_rewrite Hx; setoid_rewrite Hy; tauto.
+  Qed.
+
   Lemma M_union x y :
     x ∈' ⋃ y <-> exists z, z ∈' y /\ x ∈' z.
   Proof.
     apply (@M_ZF (fun _ => ∅) ax_union). cbn; tauto.
   Qed.
 
+  Definition union x :=
+    ⋃ x.
+
+  Instance equiv_union :
+    Proper (set_equiv ==> set_equiv) union.
+  Proof.
+    intros x x' Hx. unfold union.
+    apply M_ext; unfold set_sub.
+    all: setoid_rewrite M_union.
+    all: setoid_rewrite Hx; tauto.
+  Qed.
+
   Lemma M_power x y :
-    x ∈ PP y <-> x ⊆ y.
+    x ∈' PP y <-> x ⊆' y.
   Proof.
     apply (@M_ZF (fun _ => ∅) ax_power). cbn; tauto.
   Qed.
@@ -116,7 +150,11 @@ Section ZF.
   Instance equiv_power :
     Proper (set_equiv ==> set_equiv) power.
   Proof.
-  Admitted.
+    intros x x' Hx. unfold power.
+    apply M_ext; unfold set_sub.
+    all: setoid_rewrite M_power.
+    all: setoid_rewrite Hx; tauto.
+  Qed.
 
   Lemma M_om1 :
     M_inductive ω.
@@ -130,65 +168,9 @@ Section ZF.
     apply (@M_ZF (fun _ => ∅) ax_om2). cbn; tauto.
   Qed.
 
-  (*
-  Definition agrees_fun phi (P : V -> Prop) :=
-    forall x rho, P x <-> (x.:rho) ⊨ phi.
-
-  Definition def_pred (P : V -> Prop) :=
-    exists phi rho, forall d, P d <-> (d.:rho) ⊨ phi.
-
-  Lemma M_sep P x :
-    (forall phi rho, rho ⊨ ax_sep phi) -> def_pred P -> exists y, forall z, z ∈ y <-> z ∈ x /\ P z.
-  Proof.
-    cbn. intros H [phi [rho Hp]].
-    destruct (H phi rho x) as [y H']; clear H.
-    exists y. intros z. specialize (H' z). setoid_rewrite sat_comp in H'.
-    rewrite (sat_ext _ _ (xi:=z.:rho)) in H'; try now intros [].
-    firstorder.
-  Qed.
-
-  Definition M_is_rep R x y :=
-    forall v, v ∈ y <-> exists u, u ∈ x /\ R u v.
-
-  Lemma is_rep_unique R x y y' :
-    M_is_rep R x y -> M_is_rep R x y' -> y = y'.
-  Proof.
-    intros H1 H2. apply M_ext; intros v.
-    - intros H % H1. now apply H2.
-    - intros H % H2. now apply H1.
-  Qed.
-
-  Definition functional (R : V -> V -> Prop) :=
-    forall x y y', R x y -> R x y' -> y = y'.
-
-  Definition def_rel (R : V -> V -> Prop) :=
-    exists phi rho, forall x y, R x y <-> (x.:y.:rho) ⊨ phi.
-
-  Lemma M_rep R x :
-    (forall phi rho, rho ⊨ ax_rep phi) -> def_rel R -> functional R -> exists y, M_is_rep R x y.
-  Proof.
-    intros H1 [phi [rho Hp]]. intros H2.
-    cbn in H1. specialize (H1 phi rho). destruct H1 with x as [y Hy].
-    - intros a b b'. setoid_rewrite sat_comp.
-      erewrite sat_ext. rewrite <- (Hp a b). 2: now intros [|[]].
-      erewrite sat_ext. rewrite <- (Hp a b'). 2: now intros [|[]].
-      rewrite VIEQ. apply H2.
-    - exists y. intros v. split.
-      + intros [u[U1 U2]] % Hy. exists u. split; trivial.
-        setoid_rewrite sat_comp in U2. rewrite sat_ext in U2. rewrite (Hp u v). apply U2. now intros [|[]]; cbn.
-      + intros [u[U1 U2]]. apply Hy. exists u. split; trivial.
-        setoid_rewrite sat_comp. rewrite sat_ext. rewrite <- (Hp u v). apply U2. now intros [|[]]; cbn.
-  Qed.
-
 
 
   (* ** Basic ZF *)
-
-  Definition M_sing x :=
-    {x; x}.
-
-  Definition M_opair x y := ({{x; x}; {x; y}}).
-  *)
 
   Definition M_binunion x y :=
     ⋃ {x; y}.
@@ -209,7 +191,11 @@ Section ZF.
   Instance equiv_bunion :
     Proper (set_equiv ==> set_equiv ==> set_equiv) M_binunion.
   Proof.
-  Admitted.
+    intros x x' Hx y y' Hy. unfold M_binunion.
+    apply M_ext; unfold set_sub.
+    all: setoid_rewrite binunion_el.
+    all: setoid_rewrite Hx; setoid_rewrite Hy; tauto.
+  Qed.
 
   Lemma sing_el x y :
     x ∈' M_sing y <-> x ≡' y.
@@ -248,11 +234,6 @@ Section ZF.
     rewrite He in H. apply M_pair in H as [H|H]; apply (sing_pair H).
   Qed.
 
-  Instance set_equiv_opair :
-    Proper (set_equiv ==> set_equiv ==> set_equiv) M_opair.
-  Proof.
-  Admitted.
-
   Lemma opair_inj2 x x' y y' :
     M_opair x y ≡' M_opair x' y' -> y ≡' y'.
   Proof.
@@ -286,18 +267,6 @@ Section ZF.
       right. now apply sing_el.
   Qed.
 
-  (*Lemma sigma_eq x :
-    x ∈ σ x.
-  Proof.
-    apply sigma_el. now right.
-  Qed.
-
-  Lemma sigma_sub x :
-    x ⊆ σ x.
-  Proof.
-    intros y H. apply sigma_el. now left.
-  Qed.*)
-
   Lemma binunion_eset x :
     x ≡' ∅ ∪ x.
   Proof.
@@ -313,14 +282,6 @@ Section ZF.
   Proof.
     apply M_ext; intros z; rewrite !M_pair; tauto.
   Qed.
-
-  Definition union x :=
-    ⋃ x.
-
-  Instance equiv_union :
-    Proper (set_equiv ==> set_equiv) union.
-  Proof.
-  Admitted.
 
   Lemma binunion_com x y :
     x ∪' y ≡' y ∪' x.
@@ -350,86 +311,15 @@ Section ZF.
     - apply binunion_el in H as [H|H]; eauto.
   Qed.
 
-  
-  
-  (* ** Numerals *)
-
-  (*Fixpoint numeral n :=
-    match n with 
-    | O => ∅
-    | S n => σ (numeral n)
-    end.
-
-  Lemma numeral_omega n :
-    numeral n ∈ ω.
-  Proof.
-    induction n; cbn; now apply M_om1.
-  Qed.
-
-  Definition trans x :=
-    forall y, y ∈ x -> y ⊆ x.
-
-  Lemma numeral_trans n :
-    trans (numeral n).
-  Proof.
-    induction n; cbn.
-    - intros x H. now apply M_eset in H.
-    - intros x [H| ->] % sigma_el; try apply sigma_sub.
-      apply IHn in H. intuition eauto using sigma_sub.
-  Qed.
-
-  Lemma numeral_wf n :
-    ~ numeral n ∈ numeral n.
-  Proof.
-    induction n.
-    - apply M_eset.
-    - intros [H|H] % sigma_el; fold numeral in *.
-      + apply IHn. eapply numeral_trans; eauto. apply sigma_eq.
-      + assert (numeral n ∈ numeral (S n)) by apply sigma_eq.
-        now rewrite H in H0.
-  Qed.*)
-
   Lemma numeral_lt k l :
     k < l -> numeral k ∈ numeral l.
   Proof.
     induction 1; cbn; apply sigma_el; auto.
   Qed.
 
-  (*Lemma numeral_inj k l :
-    numeral k = numeral l -> k = l.
-  Proof.
-    intros Hk. assert (k = l \/ k < l \/ l < k) as [H|[H|H]] by lia; trivial.
-    all: apply numeral_lt in H; rewrite Hk in H; now apply numeral_wf in H.
-  Qed.
-
 
 
   (* ** Encodings *)
-
-  (* Encodings of booleans, strings, cards, and stacks *)
-
-  Definition M_enc_bool (x : bool) :=
-    if x then {∅; ∅} else ∅.
-
-  Fixpoint M_prep_string (s : string bool) x :=
-    match s with
-    | nil => x
-    | b::s => M_opair (M_enc_bool b) (M_prep_string s x)
-    end.
-
-  Definition M_enc_string (s : string bool) :=
-    M_prep_string s ∅.
-
-  Definition M_enc_card s t :=
-    M_opair (M_enc_string s) (M_enc_string t).
-
-  Fixpoint M_enc_stack (B : BSRS) :=
-    match B with
-    | nil => ∅
-    | (s,t)::B => M_enc_stack B ∪ M_sing (M_enc_card s t)
-    end.*)
-
-  (* Injectivity of encodings *)
 
   Lemma enc_bool_inj b c :
     M_enc_bool b ≡' M_enc_bool c -> b = c.
@@ -453,42 +343,13 @@ Section ZF.
       apply enc_bool_inj in H1 as ->. reflexivity.
   Qed.
 
-  (*
-  (* Agreement to syntactical encodings under evaluation *)
-
-  Lemma eval_opair rho x y :
-    eval rho (opair x y) = M_opair (eval rho x) (eval rho y).
+  Instance equiv_prep :
+    Proper (eq ==> set_equiv ==> set_equiv) M_prep_string.
   Proof.
-    reflexivity.
+    intros s s' <- x x' Hx.
+    induction s; cbn; trivial.
+    now rewrite IHs.
   Qed.
-
-  Lemma eval_enc_bool rho b :
-    eval rho (enc_bool b) = M_enc_bool b.
-  Proof.
-    destruct b; reflexivity.
-  Qed.
-
-  Lemma eval_prep_string rho s x :
-    eval rho (prep_string s x) = M_prep_string s (eval rho x).
-  Proof.
-    induction s; trivial. cbn [prep_string].
-    now rewrite eval_opair, IHs, eval_enc_bool.
-  Qed.
-
-  Lemma eval_enc_string rho s :
-    eval rho (enc_string s) = M_enc_string s.
-  Proof.
-    unfold enc_string. now rewrite eval_prep_string.
-  Qed.
-  
-  Lemma eval_enc_stack rho B :
-    eval rho (enc_stack B) = M_enc_stack B.
-  Proof.
-    induction B; cbn; trivial. destruct a. unfold M_enc_card.
-    now rewrite <- IHB, <- !eval_enc_string with (rho:=rho), <- eval_opair.
-  Qed. *)
-
-  (* Auxiliary lemmas for stack encodings *)
 
   Lemma M_enc_stack_app A B :
     M_enc_stack (A ++ B) ≡' M_enc_stack A ∪' M_enc_stack B.
@@ -520,179 +381,6 @@ Section ZF.
     - left. apply IH, H.
   Qed.
 
-  (*
-  Lemma M_prep_enc s s' :
-    M_prep_string s (M_enc_string s') = M_enc_string (s ++ s').
-  Proof.
-    induction s; cbn; trivial.
-    now rewrite IHs.
-  Qed.
-
-
-
-  (* ** Preservation direction *)
-
-  (*
-     We encode the k-step solutions of a PCP instance B as a set-theoretic function M_enc_derivations.
-     This function satisfies the conditions expressed in the reduction formula and
-     contains a solution whenever B is solvable.
-   *)
-     
-  Definition append_all A (c : card bool) :=
-    map (fun p => (fst c ++ fst p, snd c ++ snd p)) A.
-
-  Definition derivation_step B C :=
-    flat_map (append_all C) B.
-
-  Fixpoint derivations B n :=
-    match n with
-    | O => B
-    | S n => derivation_step B (derivations B n)
-    end.
-
-  Lemma derivable_derivations B s t :
-    derivable B s t -> exists n, s/t el derivations B n.
-  Proof.
-    induction 1.
-    - exists 0. apply H.
-    - destruct IHderivable as [n Hn]. exists (S n).
-      apply in_flat_map. exists (x, y). split; trivial.
-      apply in_map_iff. exists (u,v). cbn. split; trivial.
-  Qed.
-
-  Fixpoint M_enc_derivations B n :=
-    match n with 
-    | O => M_sing (M_opair ∅ (M_enc_stack B))
-    | S n => M_enc_derivations B n ∪
-            M_sing (M_opair (numeral (S n)) (M_enc_stack (derivations B (S n))))
-    end.
-
-  Lemma enc_derivations_base B n :
-    M_opair ∅ (M_enc_stack B) ∈ M_enc_derivations B n.
-  Proof.
-    induction n; cbn.
-    - now apply sing_el.
-    - apply binunion_el. now left.
-  Qed.
-
-  Lemma enc_derivations_bound B n k x :
-    M_opair k x ∈ M_enc_derivations B n -> k ∈ σ (numeral n).
-  Proof.
-    induction n; cbn.
-    - intros H % sing_el. apply opair_inj in H as [-> _].
-      apply sigma_el. now right.
-    - intros [H|H] % binunion_el.
-      + apply sigma_el. left. apply IHn, H.
-      + apply sing_el in H. apply opair_inj in H as [-> _]. apply sigma_eq.
-  Qed. 
-
-  Lemma enc_derivations_fun B n :
-    forall k x y, M_opair k x ∈ M_enc_derivations B n -> M_opair k y ∈ M_enc_derivations B n -> x = y.
-  Proof.
-    induction n; cbn -[derivations]; intros k x y.
-    - intros H1 % sing_el H2 % sing_el.
-      rewrite <- H2 in H1. now apply opair_inj in H1.
-    - intros [H1|H1 % sing_el] % binunion_el [H2|H2 % sing_el] % binunion_el.
-      + now apply (IHn k x y).
-      + exfalso. apply enc_derivations_bound in H1.
-        destruct (opair_inj H2) as [-> _]. now apply (@numeral_wf (S n)).
-      + exfalso. apply enc_derivations_bound in H2.
-        destruct (opair_inj H1) as [-> _]. now apply (@numeral_wf (S n)).
-      + rewrite <- H2 in H1. now apply opair_inj in H1.
-  Qed.
-
-  Lemma enc_derivations_el B n k x :
-    M_opair k x ∈ M_enc_derivations B n -> exists l, k = numeral l /\ x = M_enc_stack (derivations B l).
-  Proof.
-    induction n; cbn.
-    - intros H % sing_el. exists 0. apply (opair_inj H).
-    - intros [H|H] % binunion_el.
-      + apply IHn, H.
-      + apply sing_el in H. exists (S n). apply (opair_inj H).
-  Qed. 
-
-  Lemma enc_derivations_step B n l :
-    numeral l ∈ numeral n
-    -> M_opair (σ (numeral l)) (M_enc_stack (derivations B (S l))) ∈ M_enc_derivations B n.
-  Proof.
-    induction n; cbn -[derivations].
-    - now intros H % M_eset.
-    - intros [H|H % sing_el] % binunion_el; apply binunion_el.
-      + left. apply IHn, H.
-      + right. apply numeral_inj in H as ->. now apply sing_el.
-  Qed.
-
-  Lemma enc_stack_combinations B rho C x X Y :
-    rho ⊨ combinations B X Y -> eval rho X = M_enc_stack C -> eval rho Y = x -> x = M_enc_stack (derivation_step B C).
-  Proof.
-    induction B as [|[s t] B IH] in rho,C,x,X,Y |-*.
-    - cbn. rewrite VIEQ. now intros -> _ <-.
-    - intros [x1[x2[[H1 H2]H3]]] R1 R2; fold sat in *.
-      assert (x = x2 ∪ x1) as ->. { rewrite <- R2. cbn in H1. rewrite !eval_comp in H1. apply VIEQ, H1. } clear H1.
-      cbn. fold (derivation_step B C). rewrite M_enc_stack_app.
-      enough (x1 = M_enc_stack (derivation_step B C)) as E1.
-      + enough (x2 = M_enc_stack (append_all C (s / t))) as E2 by now rewrite E1, E2.
-        apply M_ext; intros u Hu.
-        * apply H3 in Hu as [v [Hv[a [b Ha]]]].
-          cbn in Hv. erewrite !eval_comp, eval_ext, R1 in Hv; trivial.
-          apply enc_stack_el' in Hv as (s'&t'&H&H').
-          enough (u = M_enc_card (s++s') (t++t')) as ->.
-          { apply enc_stack_el. apply in_map_iff. now exists (s'/t'). }
-          cbn in Ha. rewrite !VIEQ in Ha. destruct Ha as [D1 D2].
-          rewrite D1 in H'. unfold M_enc_card in H'. apply opair_inj in H' as [-> ->].
-          rewrite D2; unfold M_enc_card, M_opair; repeat f_equal.
-          all: rewrite eval_prep_string; cbn. all: apply M_prep_enc.
-        * apply enc_stack_el' in Hu as (s'&t'&H&->).
-          unfold append_all in H. eapply in_map_iff in H as [[a b][H H']].
-          cbn in H. apply H3. exists (M_enc_card a b). split.
-          { cbn. erewrite !eval_comp, eval_ext, R1; trivial. now apply enc_stack_el. }
-          exists (M_enc_string b), (M_enc_string a). split.
-          -- cbn. apply VIEQ. reflexivity.
-          -- cbn. apply VIEQ. rewrite !eval_prep_string. cbn.
-             rewrite !M_prep_enc. injection H. intros -> ->. reflexivity.
-      + eapply IH; eauto. unfold shift. now erewrite !eval_comp, eval_ext, R1.
-  Qed.
-
-  Lemma enc_derivations_solutions B n rho a b :
-    (a .: b .: M_enc_derivations B n .: numeral n .: rho) ⊨ solutions B $2 $3.
-  Proof.
-    cbn. split.
-    - rewrite eval_enc_stack. apply enc_derivations_base.
-    - intros k x x' H1 H2 H3.
-      destruct (enc_derivations_el H2) as [l[-> ->]].
-      specialize (enc_derivations_step B H1).
-      replace (M_enc_stack (derivations B (S l))) with x'; trivial.
-      apply (enc_stack_combinations H3); trivial.
-  Qed.
-
-  Lemma derivations_enc_derivations B n :
-    M_opair (numeral n) (M_enc_stack (derivations B n)) ∈ M_enc_derivations B n.
-  Proof.
-    induction n; cbn -[derivations].
-    - now apply sing_el.
-    - apply binunion_el. right.
-      now apply sing_el.
-  Qed.
-
-  Lemma derivations_el B n s t :
-     s / t el derivations B n -> M_enc_card s t ∈ M_enc_stack (derivations B n).
-  Proof.
-    apply enc_stack_el.
-  Qed.
-
-  Theorem PCP_ZF1 B s :
-    derivable B s s -> forall rho, rho ⊨ solvable B.
-  Proof.
-    intros H rho. destruct (derivable_derivations H) as [n Hn]. unfold solvable.
-    exists (numeral n), (M_enc_derivations B n), (M_enc_string s), (M_enc_stack (derivations B n)).
-    split; [split; [split; [split |] |] |].
-    - apply numeral_omega.
-    - unfold function'. intros k x y H1 H2. apply VIEQ. apply (enc_derivations_fun H1 H2).
-    - apply enc_derivations_solutions.
-    - cbn. apply derivations_enc_derivations.
-    - now apply enc_stack_el.
-  Qed.
-  *)
 
 
   (* ** Reflection direction *)
@@ -733,11 +421,6 @@ Section ZF.
 
   Definition M_solutions B f n :=
     M_opair ∅ (M_enc_stack B) ∈ f /\ forall k x y, k ∈ n -> M_opair k x ∈ f -> M_combinations B x y -> M_opair (σ k) y ∈' f.
-
-  Instance equiv_prep :
-    Proper (eq ==> set_equiv ==> set_equiv) M_prep_string.
-  Proof.
-  Admitted.
 
   Lemma comb_rel_rep C s t :
     M_is_rep (M_comb_rel s t) (M_enc_stack C) (M_enc_stack (append_all C (s, t))).
@@ -781,6 +464,7 @@ Section ZF.
   Instance equiv_solutions :
     Proper (eq ==> eq ==> set_equiv ==> iff) M_solutions.
   Proof.
+    
   Admitted.
 
   Lemma M_solutions_el B f k X p :
